\documentclass{article}
\usepackage[left=2cm,right=2cm,top=3cm,bottom=3cm]{geometry}
\usepackage{mathtools}
\usepackage{amsmath}
\usepackage{bbold}
\begin{document}
\subsubsection*{ii}
Let 
\begin{equation*}
v(x) = \int_{1}^{x} sin^{3}t \text{ } dt\\
\end{equation*}
and 
\begin{equation*}
q(x) = \int_{3}^{x}\frac{1}{1+sin^{6}t + t^2} \text{ } dt
\end{equation*}
So, $F(x) = v(q(x))$, so $\frac{dF}{dx} = \frac{dv}{dq} \frac{dq}{dx}$, so 
\begin{align*}
\frac{dF}{dx} &= \frac{1}{1+sin^{6}(x) + v^{2}} sin^{3}(x)\\
&= \frac{sin^{3}(x)}{1+sin^{6}(\int_{1}^{x} sin^{3}t \text{ } dt) + (\int_{1}^{x} sin^{3}t \text{ } dt)^{2}}
\end{align*}
\subsubsection*{iv}
\begin{align*}
F(x) &= \int_{b}^{x} \frac{1}{1+t^{2} + sin^{2}t} \quad dt\\
&= -\int_{b}^{x} \frac{1}{1+t^{2} + sin^{2}t} \quad dt\\
F^{\prime}(x) &= \frac{-1}{1+x^{2}+sin^{2}x}
\end{align*}
\subsubsection*{vi}
\begin{align*}
u(x) &= \int_{0}^{x} sin(\int_{0}^{y}sin^{3}t \quad dy)\quad dt\\
F(x) &= sin(u(x))\\
F^{\prime} &= cos(u(x))u^{\prime}\\
&= cos(\int_{0}^{x}sin(\int_{0}^{y} sin^{3} dt)dy) sin(\int_{0}^{x}sin^{3}tdt)
\end{align*}

\subsubsection*{viii}
\begin{align*}
F(F^{-1}(x)) &= x\\
\int_{0}^{F^{-1}(x)} \frac{1}{\sqrt{1-t^{2}}} dt\\
\frac{d}{dx} F(F^{-1}(x)) &= 1\\
F^{\prime}(F^{-1}(x)) F^{-1 \prime}(x)&= 1\\
\frac{1}{\sqrt{1-(F^{-1}(x))^{2})}} {F^{-1}}^{ \prime}(x)&= 1\\
{F^{-1}}^{ \prime}(x) &= \sqrt{1-(F^{-1}(x))^{2})}
\end{align*}
\end{document}
