\documentclass{article}
\usepackage[left=2cm,right=2cm,top=3cm,bottom=3cm]{geometry}
\usepackage{mathtools}
\usepackage{amsmath}
\usepackage{bbold}
\begin{document}
\subsubsection*{Q2a}
Let $y = arctan x$, then $x = tan (y) = \frac{sin y }{cos y} = \frac{sin y }{\sqrt{1-sin^{2}y}}$
\begin{align*}
x &= \frac{sin y }{\sqrt{1-sin^{2}y}}\\
x^{2} - x^{2}sin^{2}y &= sin^{2}y\\
x^{2} = sin^{2}(y) (1+x^{2}\\
sin^{2}y &= \frac{x^{2}}{1+x^{2}}\\
sin (y) &= \frac{x}{\sqrt{1+x^{2}}}
\end{align*}
For $cos(y)$:
\begin{align*}
cos(y) &= \sqrt{1-sin^{2}y}\\
&= \sqrt{1-\frac{x^{2}}{1+x^{2}}}\\
&=\sqrt{\frac{1+x^{2} - x^{2}}{1+x^{2}}}\\
&=\frac{1}{\sqrt{1+x^{2}}}
\end{align*}
\subsubsection*{Q2b}
\begin{align*}
sin(u) &= sin(2\frac{u}{2})\\
&= sin(2arctan(x))\\
&=2sin(arctan(x))cos(arctan(x))\\
&=2\frac{x}{\sqrt{1+x^{2}}}\frac{1}{\sqrt{1+x^2}}\\
&=\frac{2x}{1+x^{2}}
\end{align*}
\begin{align*}
cos(u) &= cos(2arctan(x))\\
&= 2cos^{2}(arctan(x)) - 1\\
&=\frac{2}{1+x^{2}} - 1\\
&= \frac{1-x^{2}}{1+x^{2}}
\end{align*}
\end{document}
